shallow/Proof.v
@@ -1,167 +1,393 @@
 Require Export ShallowSeparationLogic.Language.
 
-(* ============= *)
-(* SPECIFICATION *)
-(* ============= *)
+(* ========================== *)
+(* AXIOMATIC CHARACTERIZATION *)
+(* ========================== *)
 
-Inductive spec: Type :=
-| mkhoare: cassert -> program -> cassert -> spec.
-
-Definition valid (p: cassert): Prop :=
-  forall h s, p (h, s).
-
-Definition correct (psq: spec): Prop :=
-  match psq with
-  | mkhoare p S1 q =>
-    forall h s, p (h, s) ->
-      ~bigstep S1 (h, s) None /\
-      forall h' s', bigstep S1 (h, s) (Some (h', s')) -> q (h', s')
-  end.
-
-(* ======================================================================= *)
-(* WEAKEST PRECONDITION AXIOMATIZATION (WP-CSL), SEE FIGURE 3 IN THE PAPER *)
-(* ======================================================================= *)
-
-Inductive WPCSL: spec -> Type :=
-| wpc_basic (p: cassert) (x: V) (e: expr):
-    WPCSL (mkhoare (csub p x e) (basic x e) p)
-| wpc_lookup (p: cassert) (x y: V) (e: expr):
-    ~In y (x :: cvar p ++ evar e) ->
-    WPCSL (mkhoare (clexists y (cland (chasval e y) (csub p x y))) (lookup x e) p)
-| wpc_mutation (p: cassert) (x: V) (e: expr):
-    WPCSL (mkhoare (cland (chasvaldash x) (csub_heap_update p x e)) (mutation x e) p)
-| wpc_new (p: cassert) (x: V) (e: expr):
-    ~In x (evar e) ->
-    WPCSL (mkhoare (clforall x (climp (clnot (chasvaldash x)) (csub_heap_update p x e))) (new x e) p)
-| wpc_dispose (p: cassert) (x: V):
-    WPCSL (mkhoare (cland (chasvaldash x) (csub_heap_clear p x)) (dispose x) p)
-| wpc_skip (p: cassert):
-    WPCSL (mkhoare p skip p)
-| wpc_compose (p q r: cassert) (S1 S2: program):
-    WPCSL (mkhoare p S1 r) ->
-    WPCSL (mkhoare r S2 q) ->
-    WPCSL (mkhoare p (comp S1 S2) q)
-| wpc_ite (p q: cassert) (g: guard) (S1 S2: program):
-    WPCSL (mkhoare (cland p (ctest g)) S1 q) ->
-    WPCSL (mkhoare (cland p (clnot (ctest g))) S2 q) ->
-    WPCSL (mkhoare p (ite g S1 S2) q)
-| wpc_while (p: cassert) (g: guard) (S1: program):
-    WPCSL (mkhoare (cland p (ctest g)) S1 p) ->
-    WPCSL (mkhoare p (while g S1) (cland p (clnot (ctest g))))
-| wpc_conseq (p pp q qq: cassert) (x: program):
-    valid (climp pp p) -> WPCSL (mkhoare p x q) -> valid (climp q qq) ->
-    WPCSL (mkhoare pp x qq).
-
-(* Soundness of the proof system *)
-
-Proposition WPCSL_basic_soundness (p: cassert) (x: V) (e: expr):
-  correct (mkhoare (csub p x e) (basic x e) p).
-Admitted.
-
-Proposition WPCSL_lookup_soundness (p: cassert) (x y: V) (e: expr):
-  ~ In y (x :: cvar p ++ evar e) ->
-  correct (mkhoare (clexists y (cland (chasval e y) (csub p x y))) (lookup x e) p).
-Admitted.
-
-Proposition WPCSL_mutation_soundness (p: cassert) (x: V) (e: expr):
-  correct (mkhoare (cland (chasvaldash x) (csub_heap_update p x e)) (mutation x e) p).
-Admitted.
-
-Proposition WPCSL_new_soundness (p: cassert) (x: V) (e: expr):
-  ~ In x (evar e) ->
-  correct (mkhoare (clforall x (climp (clnot (chasvaldash x)) (csub_heap_update p x e))) (new x e) p).
-Admitted.
-
-Proposition WPCSL_dispose_soundness (p: cassert) (x: V):
-  correct (mkhoare (cland (chasvaldash x) (csub_heap_clear p x)) (dispose x) p).
-Admitted.
-
-Proposition WPCSL_skip_soundness (p: cassert):
-  correct (mkhoare p skip p).
-intro; intros. split.
-+ intro. inversion H0.
-+ intros. inversion H0.
-  rewrite <- H4.
-  rewrite <- H5.
-  assumption.
+(* Conjunction and program modality *)
+Lemma cwlp_cland_distr (S1: program) (p q: cassert):
+  valid (clequiv (cwlp S1 (cland p q)) (cland (cwlp S1 p) (cwlp S1 q))).
+unfold valid; intros.
+simpl. split; intros.
+- destruct H.
+  split; split; auto.
+  all: intros; apply H0; auto.
+- destruct H; destruct H; destruct H0.
+  split. auto.
+  intros. split.
+  apply H1. auto.
+  apply H2. auto.
 Qed.
 
-Proposition WPCSL_comp_soundness (p q r: cassert) (S1 S2: program):
-  correct (mkhoare p S1 r) ->
-  correct (mkhoare r S2 q) ->
-  correct (mkhoare p (comp S1 S2) q).
-intros; intro; intros. split.
-+ unfold correct in *.
-  specialize H with h s.
-  apply H in H1; clear H.
-  destruct H1.
+(* Complex programs *)
+Lemma cwlp_diverge (p: cassert):
+  valid (clequiv (cwlp diverge p) cltrue).
+unfold valid; intros.
+simpl. split; intros; auto.
+split; intro; intros; inversion H0.
+Qed.
+
+Lemma cwlp_skip (p: cassert):
+  valid (clequiv (cwlp skip p) p).
+unfold valid; intros.
+simpl. split; intros.
+- destruct H. apply H0.
+  apply step_skip.
+- split; intro; intros; inversion H0.
+  rewrite <- H4. rewrite <- H5.
+  auto.
+Qed.
+
+Lemma cwlp_comp (S1 S2: program) (p: cassert):
+  valid (clequiv (cwlp (comp S1 S2) p) (cwlp S1 (cwlp S2 p))).
+unfold valid; intros.
+simpl. split; intros.
+- destruct H. split.
+  + intro. apply H.
+    apply step_comp_fail1. auto.
+  + intros. split.
+    intro. apply H.
+    eapply step_comp_fail2. apply H1. auto.
+    intros. apply H0.
+    eapply step_comp. apply H1. apply H2.
+- destruct H. split.
+  + intro. inversion H1.
+    apply H. auto.
+    specialize H0 with h' s'.
+    apply H0 in H5. destruct H5.
+    apply H5. auto.
+  + intros. inversion H1.
+    edestruct H0. apply H5.
+    apply H11. apply H9.
+Qed.
+
+Lemma cwlp_ite (g: guard) (S1 S2: program) (p: cassert):
+  valid (clequiv (cwlp (ite g S1 S2) p) (cland (climp (ctest g) (cwlp S1 p)) (climp (clnot (ctest g)) (cwlp S2 p)))).
+unfold valid; intros.
+simpl. split; intros.
+- destruct H. split; intros.
+  + split. intro. apply H.
+    apply step_ite_true; auto.
+    intros. apply H0.
+    apply step_ite_true; auto.
+  + split. intro. apply H.
+    apply step_ite_false; auto.
+    destruct (g s); auto. symmetry; apply H1; auto.
+    intros. apply H0.
+    apply step_ite_false; auto.
+    destruct (g s); auto. symmetry; apply H1; auto.
+- destruct H.
+  split.
+  + intro. inversion H1.
+    destruct H; auto.
+    destruct H0; auto. intro.
+    destruct (g s). inversion H8. inversion H0.
+  + intros. inversion H1.
+    apply H in H8. destruct H8. apply H10. auto.
+    destruct H0. intro. destruct (g s). inversion H8. inversion H0.
+    apply H10. auto.
+Qed.
+
+Lemma cwlp_while (g: guard) (S1: program) (p q: cassert):
+  valid (clequiv (cwlp (while g S1) p) (cwlp (ite g (comp S1 (while g S1)) skip) p)).
+unfold valid; intros.
+simpl. split; intros.
+- destruct H.
+  split. intro.
+  rewrite while_unfold in H.
+  apply H; auto.
+  intros. apply H0.
+  rewrite while_unfold; auto.
+- destruct H. split.
   intro.
-  inversion H2. apply H. assumption.
-  apply H1 in H6.
-  apply H0 in H6; clear H0.
-  destruct H6.
-  apply H0; assumption.
-+ unfold correct in *.
-  specialize H with h s.
-  apply H in H1; clear H; destruct H1.
-  intros.
-  inversion H2.
-  apply H1 in H6.
-  apply H0 in H6.
-  destruct H6.
-  apply H11 in H10.
-  assumption.
+  rewrite <- while_unfold in H.
+  apply H; auto.
+  intros. apply H0.
+  rewrite <- while_unfold; auto.
 Qed.
 
-Proposition WPCSL_ite_soundness (p q: cassert) (g: guard) (S1 S2: program):
-  correct (mkhoare (cland p (ctest g)) S1 q) ->
-  correct (mkhoare (cland p (clnot (ctest g))) S2 q) ->
-  correct (mkhoare p (ite g S1 S2) q).
+(* Simple assignment, E1-4 *)
+Lemma cwlp_basic_ctest (x: V) (e: expr) (g: guard):
+  valid (clequiv (cwlp (basic x e) (ctest g)) (ctest (gsub g x e))).
+unfold valid; intros.
+simpl. split; intros.
+- destruct H.
+  specialize H0 with h (store_update s x (e s)).
+  apply H0.
+  apply step_basic.
+- split; intro; intros; inversion H0; auto.
+Qed.
+
+Lemma cwlp_basic_chasval (x: V) (e: expr) (e1 e2: expr):
+  valid (clequiv (cwlp (basic x e) (chasval e1 e2)) (chasval (esub e1 x e) (esub e2 x e))).
+unfold valid; intros.
+simpl. split; intros.
+- destruct H.
+  specialize H0 with h (store_update s x (e s)).
+  apply H0.
+  apply step_basic.
+- split. intro. inversion H0.
+  intros. inversion H0.
+  rewrite H6 in H. auto.
+Qed.
+
+Lemma cwlp_basic_climp (x: V) (e: expr) (p q: cassert):
+  valid (clequiv (cwlp (basic x e) (climp p q)) (climp (cwlp (basic x e) p) (cwlp (basic x e) q))).
+unfold valid; intros.
+simpl. split; intros.
+- destruct H; destruct H0. split; auto.
+- split. intro. inversion H0.
+  intros. destruct H.
+  split. intro. inversion H.
+  intros. inversion H.
+  inversion H0. rewrite <- H7.
+  rewrite H13. rewrite H14. auto.
+  apply H2. auto.
+Qed.
+
+Lemma cwlp_basic_clforall (x: V) (e: expr) (y: V) (p: cassert):
+  ~In y (pvar (basic x e)) ->
+  valid (clequiv (cwlp (basic x e) (clforall y p)) (clforall y (cwlp (basic x e) p))).
+intros. unfold valid; intros.
+simpl. split; intros.
+- split. intro. inversion H1.
+  intros. destruct H0.
+  pose proof (bigstep_cond (basic x e) _ _ H1 (pvar (basic x e))).
+  destruct H3 with (h := h) (s := store_update s y v) (t := s); auto.
+  intro. intro. unfold store_update.
+    destruct (Nat.eq_dec y x0). exfalso. apply H. rewrite e0; auto. auto.
+  destruct H4 with (h' := h') (s' := s'); auto. destruct H6.
+  inversion H7.
+  rewrite <- H13 in H7.
+  rewrite <- H14 in H7.
+  eapply H2 in H7.
+  inversion H1.
+  rewrite <- H19.
+  rewrite store_update_swap.
+  rewrite econd with (t := s).
+  apply H7.
+  intro; intros. unfold store_update.
+    destruct (Nat.eq_dec y x3). exfalso. apply H. rewrite e2. simpl. auto. auto.
+  intro. apply H. rewrite H8. simpl. auto.
+- split. intro. inversion H1.
+  intros. destruct H0 with (v := v).
+  specialize H3 with h (store_update (store_update s y v) x (e (store_update s y v))).
+  inversion H1.
+  rewrite store_update_swap.
+  rewrite econd with (t := (store_update s y v)).
+  rewrite <- H9. apply H3.
+  apply step_basic.
+  intro. intro. unfold store_update.
+    destruct (Nat.eq_dec y x1). exfalso. apply H. rewrite e1. simpl. auto. auto.
+  intro. apply H. rewrite H4. simpl. auto.
+Qed.
+
+Lemma cwlp_basic_csand (x: V) (e: expr) (p q: cassert):
+  valid (clequiv (cwlp (basic x e) (csand p q)) (csand (cwlp (basic x e) p) (cwlp (basic x e) q))).
+unfold valid; intros.
+simpl. split; intros.
+- destruct H.
+  intro. destruct H0 with (h' := h) (s' := store_update s x (e s)).
+  apply step_basic.
+  intros. intro. destruct H2.
+  destruct H1 with (h1 := h1) (h2 := h2).
+  split; auto.
+  destruct H3.
+  split; split.
+  intro. inversion H5.
+  intros. inversion H5.
+  rewrite <- H11. auto.
+  intro. inversion H5.
+  intros. inversion H5.
+  rewrite <- H11. auto.
+- split. intro. inversion H0.
+  intros. intro.
+  apply H. intros. intro. destruct H2. destruct H3.
+  destruct H3. destruct H4.
+  destruct H1 with (h1 := h1) (h2 := h2).
+  split. inversion H0. rewrite <- H12. auto.
+  split. apply H5. inversion H0. apply step_basic.
+  apply H6. inversion H0. apply step_basic.
+Qed.
+
+Lemma cwlp_basic_csimp (x: V) (e: expr) (p q: cassert):
+  valid (clequiv (cwlp (basic x e) (csimp p q)) (csimp (cwlp (basic x e) p) (cwlp (basic x e) q))).
+unfold valid; intros.
+simpl. split; intros.
+- destruct H.
+  specialize H2 with h (store_update s x (e s)) h'' h'.
+  pose proof (step_basic x e h s).
+  apply H2 in H3; auto.
+  split. intro. inversion H4.
+  intros. inversion H4. rewrite <- H10. auto.
+  destruct H1.
+  specialize H4 with h' (store_update s x (e s)).
+  pose proof (step_basic x e h' s).
+  apply H4 in H5. auto.
+- split. intro. inversion H0.
+  intros. inversion H0.
+  rewrite <- H8 in *. clear dependent h'.
+  rewrite <- H9 in *. clear dependent s'.
+  clear dependent x0. clear dependent e0.
+  clear dependent h0. clear dependent s0.
+  rename h'0 into h'.
+  specialize H with h'' h'.
+  apply H in H1; clear H.
+  destruct H1. apply H1.
+  apply step_basic.
+  split. intro. inversion H.
+  intros. inversion H. rewrite <- H8 in *.
+  auto.
+Qed.
+
+(* E1-3 for heap update, E9-12 *)
+Lemma csub_heap_update_ctest (x: V) (e: expr) (g: guard):
+  valid (clequiv (csub_heap_update (ctest g) x e) (ctest g)).
 Admitted.
 
-Proposition WPCSL_while_soundness (p: cassert) (g: guard) (S1: program):
-  correct (mkhoare (cland p (ctest g)) S1 p) ->
-  correct (mkhoare p (while g S1) (cland p (clnot (ctest g)))).
+Lemma csub_heap_update_chasval (x: V) (e: expr) (e1 e2: expr):
+  valid (clequiv (csub_heap_update (chasval e1 e2) x e)
+    (clor (cland (ctest (equals x e1)) (ctest (equals e2 e))) (cland (clnot (ctest (equals x e1))) (chasval e1 e2)))).
 Admitted.
 
-Proposition WPCSL_conseq_soundness (p pp q qq: cassert) (S1: program):
-  valid (climp pp p) ->
-  valid (climp q qq) ->
-  correct (mkhoare p S1 q) ->
-  correct (mkhoare pp S1 qq).
-intros. unfold correct in *; intros.
-split.
-intro.
-unfold valid in *.
-simpl in H.
-apply H in H2.
-apply H1 in H2. destruct H2.
-apply H2; auto.
+Lemma csub_heap_update_climp (x: V) (e: expr) (p q: cassert):
+  valid (clequiv (csub_heap_update (climp p q) x e) (climp (csub_heap_update p x e) (csub_heap_update q x e))).
+Admitted.
+
+Lemma csub_heap_update_clforall (x: V) (e: expr) (y: V) (p: cassert):
+  ~In y (x :: evar e) ->
+  valid (clequiv (csub_heap_update (clforall y p) x e) (clforall y (csub_heap_update p x e))).
+Admitted.
+
+Lemma csub_heap_update_csand (x: V) (e: expr) (p q: cassert):
+  valid (clequiv (csub_heap_update (csand p q) x e)
+    (clor (csand (csub_heap_update p x e) (cland q (clnot (chasvaldash x))))
+      (csand (cland p (clnot (chasvaldash x))) (csub_heap_update q x e)))).
+Admitted.
+
+Lemma csub_heap_update_csimp (x: V) (e: expr) (p q: cassert):
+  valid (clequiv (csub_heap_update (csimp p q) x e)
+    (csimp (cland p (clnot (chasvaldash x))) (csub_heap_update q x e))).
+Admitted.
+
+(* E1-3 for heap clear, E13-E16 *)
+Lemma csub_heap_clear_ctest (x: V) (g: guard):
+  valid (clequiv (csub_heap_clear (ctest g) x) (ctest g)).
+Admitted.
+
+Lemma csub_heap_clear_chasval (x: V) (e1 e2: expr):
+  valid (clequiv (csub_heap_clear (chasval e1 e2) x)
+    (cland (clnot (ctest (equals x e1))) (chasval e1 e2))).
+Admitted.
+
+Lemma csub_heap_clear_climp (x: V) (p q: cassert):
+  valid (clequiv (csub_heap_clear (climp p q) x) (climp (csub_heap_clear p x) (csub_heap_clear q x))).
+Admitted.
+
+Lemma csub_heap_clear_clforall (x: V) (y: V) (p: cassert):
+  y <> x ->
+  valid (clequiv (csub_heap_clear (clforall y p) x) (clforall y (csub_heap_clear p x))).
+Admitted.
+
+Lemma csub_heap_clear_csand (x: V) (p q: cassert):
+  valid (clequiv (csub_heap_clear (csand p q) x)
+    (csand (csub_heap_clear p x) (csub_heap_clear q x))).
+Admitted.
+
+Lemma csub_heap_clear_csimp (x: V) (p q: cassert):
+  forall y, ~In y (x :: cvar p ++ cvar q) ->
+  valid (clequiv (csub_heap_clear (csimp p q) x)
+    (cland (csimp (cland p (clnot (chasvaldash x))) (csub_heap_clear q x))
+      (clforall y (csimp (csub_heap_update p x y) (csub_heap_update q x y))))).
+Admitted.
+
+(* E5 *)
+Lemma cwlp_lookup_p1 (x: V) (e: expr) (h: heap) (s: store):
+  ~ bigstep (lookup x e) (h, s) None -> exists z, h (e s) = Some z.
 intros.
-apply H in H2.
-apply H1 in H2; destruct H2.
-apply H4 in H3.
-apply H0 in H3.
-assumption.
+remember (h (e s)). destruct o.
+exists z. auto.
+exfalso. apply H.
+apply step_lookup_fail. auto.
 Qed.
 
-Theorem WPCSL_soundness (psq: spec):
-  WPCSL psq -> correct psq.
-intro.
-induction X.
-- apply WPCSL_basic_soundness.
-- apply WPCSL_lookup_soundness; auto.
-- apply WPCSL_mutation_soundness.
-- apply WPCSL_new_soundness; auto.
-- apply WPCSL_dispose_soundness.
-- apply WPCSL_skip_soundness.
-- apply WPCSL_comp_soundness with (r := r); auto.
-- apply WPCSL_ite_soundness; auto.
-- apply WPCSL_while_soundness; auto.
-- apply WPCSL_conseq_soundness with (p := p) (q := q); auto.
+Lemma cwlp_lookup (x: V) (e: expr) (p: cassert):
+  forall y, ~In y (x :: cvar p ++ evar e) ->
+    valid (clequiv (cwlp (lookup x e) p) (clexists y (cland (chasval e y) (cwlp (basic x y) p)))).
+intros. unfold valid; intros.
+simpl. split; intros.
+- destruct H0.
+  intro.
+  pose proof (cwlp_lookup_p1 x e h s H0). destruct H3.
+  specialize H2 with x0. apply H2; clear H2. split.
+  rewrite store_update_lookup_same.
+  rewrite econd with (t := s). auto.
+  intro. intro. unfold store_update.
+    destruct (Nat.eq_dec y x1). exfalso.
+    apply H. rewrite e0. right. apply in_or_app. auto. auto.
+  split. intro. inversion H2.
+  intros. inversion H2. rewrite store_update_lookup_same.
+  rewrite <- H9.
+  rewrite store_update_swap.
+  rewrite ccond with (t := store_update s x x0).
+  apply H1.
+  apply step_lookup. auto.
+  intro. intro. unfold store_update at 1.
+    destruct (Nat.eq_dec y x2). exfalso.
+    apply H. rewrite e1. right. apply in_or_app. auto. auto.
+  intro. apply H. rewrite H4. left. auto.
+- split.
+  intro. inversion H1. apply H0; clear H0. intros. intro. destruct H0.
+  rewrite econd with (t := s) in H0. rewrite H3 in H0. inversion H0.
+  intro. intros. unfold store_update.
+    destruct (Nat.eq_dec y x1); auto. exfalso.
+    apply H. rewrite e1. right. apply in_or_app; auto.
+  intros. inversion H1. rewrite <- H7.
+  apply cstable. intro. apply H0; clear H0. intros. intro.
+    destruct H0. destruct H10.
+  apply H9.
+  rewrite ccond with (t := store_update (store_update s x v) y v0).
+  assert (v = v0).
+  { rewrite econd with (t := s) in H0.
+    rewrite H7 in H0. rewrite H0 in H3. inversion H3.
+    rewrite store_update_lookup_same. auto.
+    intro. intro. unfold store_update.
+      destruct (Nat.eq_dec y x1). exfalso. apply H.
+      rewrite e1. right. apply in_or_app. auto. auto. }
+  rewrite H12.
+  rewrite store_update_swap.
+  assert (v0 = y (store_update s y v0)).
+  { simpl. rewrite store_update_lookup_same. auto. }
+  rewrite H13 at 2.
+  apply H11.
+  apply step_basic.
+  intro. apply H. rewrite H13. left; auto.
+  intro. intros. unfold store_update at 2.
+    destruct (Nat.eq_dec y x1). exfalso. apply H. rewrite e1.
+    right. apply in_or_app; auto.
+    auto.
 Qed.
 
-(* Completeness of the proof system *)
+(* E6 *)
+Lemma cwlp_mutation (x: V) (e: expr) (p: cassert):
+  valid (clequiv (cwlp (mutation x e) p) (cland (chasvaldash x) (csub_heap_update p x e))).
+Admitted.
+
+(* E7 *)
+Lemma cwlp_new (x: V) (e: expr) (p: cassert):
+  valid (clequiv (cwlp (new x e) p) (clforall x (climp (clnot (chasvaldash x)) (csub_heap_update p x e)))).
+Admitted.
+
+(* E8 *)
+Lemma cwlp_dispose (x: V) (p: cassert):
+  valid (clequiv (cwlp (dispose x) p) (cland (chasvaldash x) (csub_heap_clear p x))).
+Admitted.
+
+
+
+
+
+
 
 
 
